Wrote up name-removal

03Debruijn/NameRemoval.thy
@@ -4,62 +4,55 @@ begin
 
 subsection \<open>Name-Removal\<close>
 
-text \<open>Now, we  \<close>
+text \<open>Now, we define our conversion from named to Debruijn languages. We accumulate a naming context 
+of variables, and use their positions in the context to determine their associated index.\<close>
 
-primrec convert' :: "var list \<Rightarrow> ty expr\<^sub>s \<Rightarrow> expr\<^sub>d" where
-  "convert' \<Phi> (Var\<^sub>s x) = Var\<^sub>d (the (idx_of \<Phi> x))"
-| "convert' \<Phi> (Const\<^sub>s k) = Const\<^sub>d k"
-| "convert' \<Phi> (Lam\<^sub>s x t e) = Lam\<^sub>d t (convert' (insert_at 0 x \<Phi>) e)"
-| "convert' \<Phi> (App\<^sub>s e\<^sub>1 e\<^sub>2) = App\<^sub>d (convert' \<Phi> e\<^sub>1) (convert' \<Phi> e\<^sub>2)"
+primrec unname' :: "var list \<Rightarrow> ty expr\<^sub>s \<Rightarrow> expr\<^sub>d" where
+  "unname' \<Phi> (Var\<^sub>s x) = Var\<^sub>d (the (idx_of \<Phi> x))"
+| "unname' \<Phi> (Const\<^sub>s k) = Const\<^sub>d k"
+| "unname' \<Phi> (Lam\<^sub>s x t e\<^sub>t) = Lam\<^sub>d t (unname' (insert_at 0 x \<Phi>) e\<^sub>t)"
+| "unname' \<Phi> (App\<^sub>s e\<^sub>t\<^sub>1 e\<^sub>t\<^sub>2) = App\<^sub>d (unname' \<Phi> e\<^sub>t\<^sub>1) (unname' \<Phi> e\<^sub>t\<^sub>2)"
 
-definition convert :: "ty expr\<^sub>s \<Rightarrow> expr\<^sub>d" where
-  "convert e \<equiv> convert' [] e"
+text \<open>The unnaming operation commutes with the various operations on expressions as we would expect 
+it to. In particular, it connects capture-avoiding substitution and the simpler Debruijn 
+substitution (see \<open>unname_subst\<close>).\<close>
 
-lemma [simp]: "value\<^sub>s e \<Longrightarrow> value\<^sub>d (convert' \<Phi> e)"
-  by (induction e) (simp_all add: Let_def)
-
-lemma [simp]: "y \<notin> all_vars\<^sub>s e \<Longrightarrow> x \<le> length \<Phi> \<Longrightarrow> free_vars\<^sub>s e \<subseteq> set \<Phi> \<Longrightarrow>
-  convert' (insert_at x y \<Phi>) e = incr\<^sub>d x (convert' \<Phi> e)"
-proof (induction e arbitrary: x \<Phi>)
+lemma unname_insert_at [simp]: "y \<notin> all_vars\<^sub>s e\<^sub>t \<Longrightarrow> x \<le> length \<Phi> \<Longrightarrow> free_vars\<^sub>s e\<^sub>t \<subseteq> set \<Phi> \<Longrightarrow>
+  unname' (insert_at x y \<Phi>) e\<^sub>t = incr\<^sub>d x (unname' \<Phi> e\<^sub>t)"
+proof (induction e\<^sub>t arbitrary: x \<Phi>)
   case (Var\<^sub>s z)
   moreover then obtain w where "idx_of \<Phi> z = Some w" by fastforce
   ultimately show ?case by simp
 next
-  case (Lam\<^sub>s z t e)
-  moreover hence "free_vars\<^sub>s e \<subseteq> set (insert_at 0 z \<Phi>)" by auto
+  case (Lam\<^sub>s z t e\<^sub>t)
+  moreover hence "free_vars\<^sub>s e\<^sub>t \<subseteq> set (insert_at 0 z \<Phi>)" by auto
   ultimately show ?case by simp
 qed simp_all
 
-lemma [simp]: "x' \<notin> all_vars\<^sub>s e \<Longrightarrow> a \<le> length \<Phi> \<Longrightarrow> idx_of \<Phi> x = Some y \<Longrightarrow> a > y \<Longrightarrow> 
-    convert' (insert_at a x \<Phi>) e = convert' (insert_at a x' \<Phi>) e"
-  by (induction e arbitrary: a \<Phi> y) (auto simp add: incr_min split: option.splits)
+lemma unname_insert_at_irrelevant [simp]: "x' \<notin> all_vars\<^sub>s e\<^sub>t \<Longrightarrow> y \<le> length \<Phi> \<Longrightarrow> 
+    \<not>y precedes x in \<Phi> \<Longrightarrow> unname' (insert_at y x \<Phi>) e\<^sub>t = unname' (insert_at y x' \<Phi>) e\<^sub>t"
+  by (induction e\<^sub>t arbitrary: y \<Phi>) (auto simp add: incr_min split: option.splits)
 
-abbreviation precede :: "nat \<Rightarrow> 'a \<Rightarrow> 'a list \<Rightarrow> bool" (infix "precedes _ in" 50) where
-  "x precedes a in as \<equiv> (case idx_of as a of Some y \<Rightarrow> x \<le> y | None \<Rightarrow> True)"
-
-lemma [simp]: "0 precedes a in as"
-  by (simp split: option.splits)
-
-lemma [simp]: "y \<le> length \<Phi> \<Longrightarrow> y precedes x in \<Phi> \<Longrightarrow> y precedes x' in \<Phi> \<Longrightarrow> x' \<notin> all_vars\<^sub>s e \<Longrightarrow> 
-  free_vars\<^sub>s e \<subseteq> insert x (set \<Phi>) \<Longrightarrow> 
-    convert' (insert_at y x' \<Phi>) (subst_var\<^sub>s x x' e) = convert' (insert_at y x \<Phi>) e"
-proof (induction e arbitrary: y \<Phi>)
-  case (Lam\<^sub>s z t e)
+lemma unname_subst_var [simp]: "y \<le> length \<Phi> \<Longrightarrow> y precedes x in \<Phi> \<Longrightarrow> y precedes x' in \<Phi> \<Longrightarrow> 
+  x' \<notin> all_vars\<^sub>s e\<^sub>t \<Longrightarrow> free_vars\<^sub>s e\<^sub>t \<subseteq> insert x (set \<Phi>) \<Longrightarrow> 
+    unname' (insert_at y x' \<Phi>) (subst_var\<^sub>s x x' e\<^sub>t) = unname' (insert_at y x \<Phi>) e\<^sub>t"
+proof (induction e\<^sub>t arbitrary: y \<Phi>)
+  case (Lam\<^sub>s z t e\<^sub>t)
   thus ?case
   proof (cases "x = z")
     case False
     with Lam\<^sub>s have X: "Suc y precedes x in insert_at 0 z \<Phi>" by (simp split: option.splits) 
     from Lam\<^sub>s have Y: "Suc y precedes x' in insert_at 0 z \<Phi>" by (simp split: option.splits) 
-    from Lam\<^sub>s have "free_vars\<^sub>s e \<subseteq> insert x (set (insert_at 0 z \<Phi>))" by auto
+    from Lam\<^sub>s have "free_vars\<^sub>s e\<^sub>t \<subseteq> insert x (set (insert_at 0 z \<Phi>))" by auto
     with Lam\<^sub>s False X Y show ?thesis by simp
   qed (simp_all split: option.splits)
 qed (auto split: option.splits)
 
-lemma convert_subst [simp]: "y \<le> length \<Phi> \<Longrightarrow> x \<notin> set \<Phi> \<Longrightarrow> free_vars\<^sub>s e \<subseteq> insert x (set \<Phi>) \<Longrightarrow>
-  free_vars\<^sub>s e' \<subseteq> set \<Phi> \<Longrightarrow>
-    convert' \<Phi> (subst\<^sub>s x e' e) = subst\<^sub>d y (convert' \<Phi> e') (convert' (insert_at y x \<Phi>) e)" 
-proof (induction x e' e arbitrary: \<Phi> y rule: subst\<^sub>s.induct)
-  case (1 x e' z)
+lemma unname_subst [simp]: "y \<le> length \<Phi> \<Longrightarrow> x \<notin> set \<Phi> \<Longrightarrow> free_vars\<^sub>s e\<^sub>t \<subseteq> insert x (set \<Phi>) \<Longrightarrow>
+  free_vars\<^sub>s e\<^sub>t' \<subseteq> set \<Phi> \<Longrightarrow>
+    unname' \<Phi> (subst\<^sub>s x e\<^sub>t' e\<^sub>t) = subst\<^sub>d y (unname' \<Phi> e\<^sub>t') (unname' (insert_at y x \<Phi>) e\<^sub>t)" 
+proof (induction x e\<^sub>t' e\<^sub>t arbitrary: \<Phi> y rule: subst\<^sub>s.induct)
+  case (1 x e\<^sub>t' z)
   thus ?case
   proof (cases "idx_of \<Phi> z")
     case (Some w)
@@ -67,149 +60,173 @@ proof (induction x e' e arbitrary: \<Phi> y rule: subst\<^sub>s.induct)
     with 1 Some show ?thesis by auto
   qed simp_all
 next
-  case (3 x e' z t e)
-  let ?z' = "fresh (all_vars\<^sub>s e' \<union> all_vars\<^sub>s e \<union> {x, z})"
-  have "finite (all_vars\<^sub>s e' \<union> all_vars\<^sub>s e \<union> {x, z})" by simp
-  hence Z: "?z' \<notin> all_vars\<^sub>s e' \<union> all_vars\<^sub>s e \<union> {x, z}" by (metis fresh_is_fresh)
-  from 3 Z have X: "free_vars\<^sub>s e' \<subseteq> set (insert_at 0 ?z' \<Phi>)" by auto
-  from 3 have "free_vars\<^sub>s e \<subseteq> insert z (insert x (set \<Phi>))" by auto
-  with Z have "free_vars\<^sub>s (subst_var\<^sub>s z ?z' e) \<subseteq> insert ?z' (insert x (set \<Phi>))" by auto
-  hence "free_vars\<^sub>s (subst_var\<^sub>s z ?z' e) \<subseteq> insert x (set (insert_at 0 ?z' \<Phi>))" by auto
-  with 3 X Z have H: "convert' (insert_at 0 ?z' \<Phi>) (subst\<^sub>s x e' (subst_var\<^sub>s z ?z' e)) = 
-    subst\<^sub>d (Suc y) (convert' (insert_at 0 ?z' \<Phi>) e') 
-      (convert' (insert_at (Suc y) x (insert_at 0 ?z' \<Phi>)) (subst_var\<^sub>s z ?z' e))" by fastforce
-  from 3 have "free_vars\<^sub>s e \<subseteq> insert z (set (insert_at y x \<Phi>))" by auto
-  with Z have "convert' (insert_at 0 ?z' (insert_at y x \<Phi>)) (subst_var\<^sub>s z ?z' e) =
-    convert' (insert_at 0 z (insert_at y x \<Phi>)) e" by simp
+  case (3 x e\<^sub>t' z t e\<^sub>t)
+  let ?z' = "fresh (all_vars\<^sub>s e\<^sub>t' \<union> all_vars\<^sub>s e\<^sub>t \<union> {x, z})"
+  have "finite (all_vars\<^sub>s e\<^sub>t' \<union> all_vars\<^sub>s e\<^sub>t \<union> {x, z})" by simp
+  hence Z: "?z' \<notin> all_vars\<^sub>s e\<^sub>t' \<union> all_vars\<^sub>s e\<^sub>t \<union> {x, z}" by (metis fresh_is_fresh)
+  from 3 Z have X: "free_vars\<^sub>s e\<^sub>t' \<subseteq> set (insert_at 0 ?z' \<Phi>)" by auto
+  from 3 have "free_vars\<^sub>s e\<^sub>t \<subseteq> insert z (insert x (set \<Phi>))" by auto
+  with Z have "free_vars\<^sub>s (subst_var\<^sub>s z ?z' e\<^sub>t) \<subseteq> insert ?z' (insert x (set \<Phi>))" by auto
+  hence "free_vars\<^sub>s (subst_var\<^sub>s z ?z' e\<^sub>t) \<subseteq> insert x (set (insert_at 0 ?z' \<Phi>))" by auto
+  with 3 X Z have H: "unname' (insert_at 0 ?z' \<Phi>) (subst\<^sub>s x e\<^sub>t' (subst_var\<^sub>s z ?z' e\<^sub>t)) = 
+    subst\<^sub>d (Suc y) (unname' (insert_at 0 ?z' \<Phi>) e\<^sub>t') 
+      (unname' (insert_at (Suc y) x (insert_at 0 ?z' \<Phi>)) (subst_var\<^sub>s z ?z' e\<^sub>t))" by fastforce
+  from 3 have "free_vars\<^sub>s e\<^sub>t \<subseteq> insert z (set (insert_at y x \<Phi>))" by auto
+  with Z have "unname' (insert_at 0 ?z' (insert_at y x \<Phi>)) (subst_var\<^sub>s z ?z' e\<^sub>t) =
+    unname' (insert_at 0 z (insert_at y x \<Phi>)) e\<^sub>t" by simp
   with 3 Z H show ?case by (simp add: Let_def)
 qed simp_all
 
-theorem correctnd [simp]: "e \<Down>\<^sub>s v \<Longrightarrow> free_vars\<^sub>s e = {} \<Longrightarrow> convert e \<Down>\<^sub>d convert v"
-proof (induction e v rule: eval\<^sub>s.induct)
-  case (ev\<^sub>s_app e\<^sub>1 x t e\<^sub>1' e\<^sub>2 v\<^sub>2 v)
-  hence "e\<^sub>1 \<Down>\<^sub>s Lam\<^sub>s x t e\<^sub>1'" by simp
-  moreover from ev\<^sub>s_app have "free_vars\<^sub>s e\<^sub>1 = {}" by simp
-  ultimately have "free_vars\<^sub>s (Lam\<^sub>s x t e\<^sub>1') = {}" by (metis free_vars_eval)
-  hence X: "free_vars\<^sub>s e\<^sub>1' \<subseteq> insert x (set [])" by simp
-  moreover from ev\<^sub>s_app have Y: "free_vars\<^sub>s v\<^sub>2 \<subseteq> set []" by simp
-  ultimately have "free_vars\<^sub>s (subst\<^sub>s x v\<^sub>2 e\<^sub>1') \<subseteq> set []" by (metis free_vars_subst)
-  with ev\<^sub>s_app X Y show ?case by (simp add: convert_def)
-qed (simp_all add: convert_def)
+text \<open>The unnaming operation ignores alpha-conversion, as we would expect.\<close>
 
-lemma [simp]: "value\<^sub>d (convert' \<Phi> e) \<Longrightarrow> value\<^sub>s e"
-  by (induction e) (simp_all add: Let_def)
-
-lemma convert_val_back: "value\<^sub>d (convert e) \<Longrightarrow> value\<^sub>s e"
-  by (simp add: convert_def)
-
-lemma [dest]: "App\<^sub>d e\<^sub>d\<^sub>1 e\<^sub>d\<^sub>2 = convert e\<^sub>n \<Longrightarrow> 
-    \<exists>e\<^sub>n\<^sub>1 e\<^sub>n\<^sub>2. e\<^sub>n = App\<^sub>s e\<^sub>n\<^sub>1 e\<^sub>n\<^sub>2 \<and> e\<^sub>d\<^sub>1 = convert e\<^sub>n\<^sub>1 \<and> e\<^sub>d\<^sub>2 = convert e\<^sub>n\<^sub>2"
-  by (cases e\<^sub>n) (simp_all add: convert_def)
-
-lemma [dest]: "Lam\<^sub>d t e\<^sub>d = convert e\<^sub>n \<Longrightarrow> 
-    \<exists>x e\<^sub>n'. e\<^sub>n = Lam\<^sub>s x t e\<^sub>n' \<and> e\<^sub>d = convert' [x] e\<^sub>n'"
-  by (cases e\<^sub>n) (simp_all add: convert_def)
-
-theorem completend [simp]: "convert e\<^sub>n \<Down>\<^sub>d v\<^sub>d \<Longrightarrow> free_vars\<^sub>s e\<^sub>n = {} \<Longrightarrow> 
-  \<exists>v\<^sub>n. e\<^sub>n \<Down>\<^sub>s v\<^sub>n \<and> v\<^sub>d = convert v\<^sub>n"
-proof (induction "convert e\<^sub>n" v\<^sub>d arbitrary: e\<^sub>n rule: big_eval\<^sub>d.induct)
-  case (bev\<^sub>d_const k)
-  hence "e\<^sub>n \<Down>\<^sub>s Const\<^sub>s k \<and> Const\<^sub>d k = convert (Const\<^sub>s k)" by (cases e\<^sub>n) (simp_all add: convert_def)
-  thus ?case by fastforce
-next
-  case (bev\<^sub>d_lam t e)
-  then obtain x e' where "e\<^sub>n = Lam\<^sub>s x t e' \<and> e = convert' [x] e'" 
-    by (cases e\<^sub>n) (simp_all add: convert_def)
-  hence "e\<^sub>n \<Down>\<^sub>s Lam\<^sub>s x t e' \<and> Lam\<^sub>d t e = convert (Lam\<^sub>s x t e')" by (simp add: convert_def)
-  thus ?case by fastforce
-next
-  case (bev\<^sub>d_app e\<^sub>1 t e\<^sub>1' e\<^sub>2 v\<^sub>2 v)
-  then obtain e\<^sub>n\<^sub>1 e\<^sub>n\<^sub>2 where E: "e\<^sub>n = App\<^sub>s e\<^sub>n\<^sub>1 e\<^sub>n\<^sub>2 \<and> e\<^sub>1 = convert e\<^sub>n\<^sub>1 \<and> e\<^sub>2 = convert e\<^sub>n\<^sub>2" 
-    by (cases e\<^sub>n) (simp_all add: convert_def)
-  with bev\<^sub>d_app obtain v\<^sub>n\<^sub>1 where V1: "e\<^sub>n\<^sub>1 \<Down>\<^sub>s v\<^sub>n\<^sub>1 \<and> Lam\<^sub>d t e\<^sub>1' = convert v\<^sub>n\<^sub>1" by fastforce
-  then obtain x e\<^sub>n\<^sub>1' where X: "v\<^sub>n\<^sub>1 = Lam\<^sub>s x t e\<^sub>n\<^sub>1' \<and> e\<^sub>1' = convert' [x] e\<^sub>n\<^sub>1'"
-    by (cases v\<^sub>n\<^sub>1) (simp_all add: convert_def)
-  from bev\<^sub>d_app E obtain v\<^sub>n\<^sub>2 where V2: "e\<^sub>n\<^sub>2 \<Down>\<^sub>s v\<^sub>n\<^sub>2 \<and> v\<^sub>2 = convert v\<^sub>n\<^sub>2" by fastforce
-  from bev\<^sub>d_app E have "free_vars\<^sub>s e\<^sub>n\<^sub>1 = {}" by simp
-  with V1 X have "free_vars\<^sub>s (Lam\<^sub>s x t e\<^sub>n\<^sub>1') = {}" by (metis free_vars_eval)
-  hence Y: "free_vars\<^sub>s e\<^sub>n\<^sub>1' \<subseteq> {x}" by simp
-  from bev\<^sub>d_app E have "free_vars\<^sub>s e\<^sub>n\<^sub>2 = {}" by simp
-  with V2 have Z: "free_vars\<^sub>s v\<^sub>n\<^sub>2 = {}" by auto
-  with Y have "free_vars\<^sub>s (subst\<^sub>s x v\<^sub>n\<^sub>2 e\<^sub>n\<^sub>1') = {}" by (metis free_vars_subst subset_empty)
-  with bev\<^sub>d_app X V2 Y Z have "\<exists>v\<^sub>n. subst\<^sub>s x v\<^sub>n\<^sub>2 e\<^sub>n\<^sub>1' \<Down>\<^sub>s v\<^sub>n \<and> v = convert v\<^sub>n" 
-    by (simp add: convert_def)
-  then obtain v\<^sub>n where "subst\<^sub>s x v\<^sub>n\<^sub>2 e\<^sub>n\<^sub>1' \<Down>\<^sub>s v\<^sub>n \<and> v = convert v\<^sub>n" by fastforce
-  with V1 X V2 have "App\<^sub>s e\<^sub>n\<^sub>1 e\<^sub>n\<^sub>2 \<Down>\<^sub>s v\<^sub>n \<and> v = convert v\<^sub>n" by fastforce
-  with E show ?case by fastforce
-qed
-
-
-(* typesafety *)
-
-lemma convert_remove_shadows [simp]: "finite vs \<Longrightarrow> free_vars\<^sub>s e \<subseteq> set \<Phi> \<Longrightarrow>
-  convert' \<Phi> (remove_shadows\<^sub>s' vs e) = convert' \<Phi> e"
-proof (induction e arbitrary: \<Phi> vs)
-  case (Lam\<^sub>s x t e)
-  let ?e = "remove_shadows\<^sub>s' (insert x vs) e"
+lemma unname_remove_shadows [simp]: "finite vs \<Longrightarrow> free_vars\<^sub>s e\<^sub>t \<subseteq> set \<Phi> \<Longrightarrow>
+  unname' \<Phi> (remove_shadows\<^sub>s' vs e\<^sub>t) = unname' \<Phi> e\<^sub>t"
+proof (induction e\<^sub>t arbitrary: \<Phi> vs)
+  case (Lam\<^sub>s x t e\<^sub>t)
+  let ?e = "remove_shadows\<^sub>s' (insert x vs) e\<^sub>t"
   let ?x = "fresh (vs \<union> all_vars\<^sub>s ?e)"
   from Lam\<^sub>s have "finite (vs \<union> all_vars\<^sub>s ?e)" by simp
   hence X: "?x \<notin> vs \<union> all_vars\<^sub>s ?e" by (metis fresh_is_fresh)
-  from Lam\<^sub>s have "free_vars\<^sub>s e \<subseteq> insert x (set \<Phi>)" by auto
+  from Lam\<^sub>s have "free_vars\<^sub>s e\<^sub>t \<subseteq> insert x (set \<Phi>)" by auto
   with Lam\<^sub>s X show ?case by (simp add: Let_def)
 qed simp_all
- 
-lemma typesafe\<^sub>d' [simp]: "\<Gamma> \<turnstile>\<^sub>t e : t \<Longrightarrow> dom \<Gamma> = set \<Phi> \<Longrightarrow> bound_vars\<^sub>s e \<inter> set \<Phi> = {} \<Longrightarrow> 
-  no_shadowing\<^sub>s e \<Longrightarrow> map (the \<circ> \<Gamma>) \<Phi> \<turnstile>\<^sub>d convert' \<Phi> e : t"
-proof (induction \<Gamma> e t arbitrary: \<Phi> rule: typing\<^sub>t.induct)
+
+text \<open>The unnaming operation is also typesafe. (We need the no-shadowing condition to make the 
+induction work, but fortunately \<open>unname_remove_shadows\<close> will let us eliminate it as a top-level 
+precondition.)\<close>
+
+lemma typesafe\<^sub>d' [simp]: "\<Gamma> \<turnstile>\<^sub>t e\<^sub>t : t \<Longrightarrow> dom \<Gamma> = set \<Phi> \<Longrightarrow> bound_vars\<^sub>s e\<^sub>t \<inter> set \<Phi> = {} \<Longrightarrow> 
+  no_shadowing\<^sub>s e\<^sub>t \<Longrightarrow> map (the \<circ> \<Gamma>) \<Phi> \<turnstile>\<^sub>d unname' \<Phi> e\<^sub>t : t"
+proof (induction \<Gamma> e\<^sub>t t arbitrary: \<Phi> rule: typing\<^sub>t.induct)
   case (tc\<^sub>t_var \<Gamma> x t)
   hence "x \<in> set \<Phi>" by auto
   with tc\<^sub>t_var show ?case by auto
 next
-  case (tc\<^sub>t_lam \<Gamma> x t\<^sub>1 e t\<^sub>2)
+  case (tc\<^sub>t_lam \<Gamma> x t\<^sub>1 e\<^sub>t t\<^sub>2)
   moreover hence "dom (\<Gamma>(x \<mapsto> t\<^sub>1)) = set (insert_at 0 x \<Phi>)" by simp
-  moreover from tc\<^sub>t_lam have "bound_vars\<^sub>s e \<inter> set (insert_at 0 x \<Phi>) = {}" by simp
-  moreover from tc\<^sub>t_lam have "no_shadowing\<^sub>s e" by simp
-  ultimately have "map (the \<circ> \<Gamma>(x \<mapsto> t\<^sub>1)) (insert_at 0 x \<Phi>) \<turnstile>\<^sub>d convert' (insert_at 0 x \<Phi>) e : t\<^sub>2" 
+  moreover from tc\<^sub>t_lam have "bound_vars\<^sub>s e\<^sub>t \<inter> set (insert_at 0 x \<Phi>) = {}" by simp
+  moreover from tc\<^sub>t_lam have "no_shadowing\<^sub>s e\<^sub>t" by simp
+  ultimately have "map (the \<circ> \<Gamma>(x \<mapsto> t\<^sub>1)) (insert_at 0 x \<Phi>) \<turnstile>\<^sub>d unname' (insert_at 0 x \<Phi>) e\<^sub>t : t\<^sub>2" 
     by blast
-  with tc\<^sub>t_lam have "map (the \<circ> \<Gamma>) \<Phi> \<turnstile>\<^sub>d convert' \<Phi> (Lam\<^sub>s x t\<^sub>1 e) : Arrow t\<^sub>1 t\<^sub>2" by simp
+  with tc\<^sub>t_lam have "map (the \<circ> \<Gamma>) \<Phi> \<turnstile>\<^sub>d unname' \<Phi> (Lam\<^sub>s x t\<^sub>1 e\<^sub>t) : Arrow t\<^sub>1 t\<^sub>2" by simp
   thus ?case by blast
 next
-  case (tc\<^sub>t_app \<Gamma> e\<^sub>1 t\<^sub>1 t\<^sub>2 e\<^sub>2)
-  moreover hence "bound_vars\<^sub>s e\<^sub>1 \<inter> set \<Phi> = {}" by auto
-  ultimately have T: "map (the \<circ> \<Gamma>) \<Phi> \<turnstile>\<^sub>d convert' \<Phi> e\<^sub>1 : Arrow t\<^sub>1 t\<^sub>2" by fastforce
-  from tc\<^sub>t_app have "bound_vars\<^sub>s e\<^sub>2 \<inter> set \<Phi> = {}" by auto
-  with tc\<^sub>t_app have "map (the \<circ> \<Gamma>) \<Phi> \<turnstile>\<^sub>d convert' \<Phi> e\<^sub>2 : t\<^sub>1" by fastforce
-  with T have "map (the \<circ> \<Gamma>) \<Phi> \<turnstile>\<^sub>d convert' \<Phi> (App\<^sub>s e\<^sub>1 e\<^sub>2) : t\<^sub>2" by simp
+  case (tc\<^sub>t_app \<Gamma> e\<^sub>t\<^sub>1 t\<^sub>1 t\<^sub>2 e\<^sub>t\<^sub>2)
+  moreover hence "bound_vars\<^sub>s e\<^sub>t\<^sub>1 \<inter> set \<Phi> = {}" by auto
+  ultimately have T: "map (the \<circ> \<Gamma>) \<Phi> \<turnstile>\<^sub>d unname' \<Phi> e\<^sub>t\<^sub>1 : Arrow t\<^sub>1 t\<^sub>2" by fastforce
+  from tc\<^sub>t_app have "bound_vars\<^sub>s e\<^sub>t\<^sub>2 \<inter> set \<Phi> = {}" by auto
+  with tc\<^sub>t_app have "map (the \<circ> \<Gamma>) \<Phi> \<turnstile>\<^sub>d unname' \<Phi> e\<^sub>t\<^sub>2 : t\<^sub>1" by fastforce
+  with T have "map (the \<circ> \<Gamma>) \<Phi> \<turnstile>\<^sub>d unname' \<Phi> (App\<^sub>s e\<^sub>t\<^sub>1 e\<^sub>t\<^sub>2) : t\<^sub>2" by simp
   thus ?case by blast
 qed simp_all
 
-theorem typesafend [simp]: "Map.empty \<turnstile>\<^sub>t e : t \<Longrightarrow> [] \<turnstile>\<^sub>d convert e : t"
+text \<open>The full unnaming of closed terms operation follows immediately, and we can use it to prove 
+our correctness theorems.\<close>
+
+text \<open>Since this is the first full conversion we have done, we will take a moment to explain exactly 
+what we prove. There are three theorems for the conversion: typesafety, showing that any well-typed 
+abstract state is converted to a well-typed concrete state; correctness proper, showing that if an 
+abstract state evaluates to some value, then the concrete version of that state evaluates to the 
+concrete version of that value; and completeness, showing that if the concrete version of an state 
+evaluates to the concrete version of a value, then the abstract state evaluates to the abstract 
+value. (At the moment, our states are just expressions, but they will get more complicated as we 
+go on.) As mentioned in the introduction, there are complications, particularly with correctness, 
+since our conversion function often runs the other direction, and we have to prove a number of 
+reconstruction lemmas to determine what an appropriate abstract state had to have been. (In the 
+present stage, \<open>unname_to_app\<close> and \<open>unname_to_lam\<close> are our reconstruction lemmas; since this stage's 
+conversion runs "the right direction", they are needed for completeness rather than correctness.) We 
+also do not prove all the theorems for all the stages, since the execution model gets less 
+structured as we go along: once we reach Tree Code (stage 6) we no longer have a typing judgement, 
+so typesafety is lost, and once we reach Assembly (stage 13), the complexity of the reconstruction 
+lemmas required becomes so large that we abandon completeness as well. We always prove correctness, 
+of course, because composing all our correctness theorems is exactly what gives us our ultimate 
+correctness proof.\<close>
+
+definition unname :: "ty expr\<^sub>s \<Rightarrow> expr\<^sub>d" where
+  "unname e\<^sub>t \<equiv> unname' [] e\<^sub>t"
+
+theorem typesafe\<^sub>d [simp]: "Map.empty \<turnstile>\<^sub>t e\<^sub>t : t \<Longrightarrow> [] \<turnstile>\<^sub>d unname e\<^sub>t : t"
 proof -
-  assume T: "Map.empty \<turnstile>\<^sub>t e : t"
-  hence "Map.empty \<turnstile>\<^sub>t remove_shadows\<^sub>s e : t" by simp
-  moreover have "bound_vars\<^sub>s (remove_shadows\<^sub>s e) \<inter> set [] = {}" by simp
-  moreover have "no_shadowing\<^sub>s (remove_shadows\<^sub>s e)" by simp
-  ultimately have "[] \<turnstile>\<^sub>d convert' [] (remove_shadows\<^sub>s e) : t" 
+  assume T: "Map.empty \<turnstile>\<^sub>t e\<^sub>t : t"
+  hence "Map.empty \<turnstile>\<^sub>t remove_shadows\<^sub>s e\<^sub>t : t" by simp
+  moreover have "bound_vars\<^sub>s (remove_shadows\<^sub>s e\<^sub>t) \<inter> set [] = {}" by simp
+  moreover have "no_shadowing\<^sub>s (remove_shadows\<^sub>s e\<^sub>t)" by simp
+  ultimately have "[] \<turnstile>\<^sub>d unname' [] (remove_shadows\<^sub>s e\<^sub>t) : t" 
     by (metis typesafe\<^sub>d' dom_empty empty_set list.simps(8))
-  with T show ?thesis by (simp add: convert_def remove_shadows\<^sub>s_def)
+  with T show ?thesis by (simp add: unname_def remove_shadows\<^sub>s_def)
 qed
 
-(* Now we can finish the deferred progress lemmas from 01Source/Named and 02Typed/Typed *)
+theorem correct\<^sub>d [simp]: "e\<^sub>t \<Down>\<^sub>s v\<^sub>s \<Longrightarrow> free_vars\<^sub>s e\<^sub>t = {} \<Longrightarrow> unname e\<^sub>t \<Down>\<^sub>d unname v\<^sub>s"
+proof (induction e\<^sub>t v\<^sub>s rule: eval\<^sub>s.induct)
+  case (ev\<^sub>s_app e\<^sub>t\<^sub>1 x t e\<^sub>t\<^sub>1' e\<^sub>t\<^sub>2 v\<^sub>s\<^sub>2 v\<^sub>s)
+  hence "e\<^sub>t\<^sub>1 \<Down>\<^sub>s Lam\<^sub>s x t e\<^sub>t\<^sub>1'" by simp
+  moreover from ev\<^sub>s_app have "free_vars\<^sub>s e\<^sub>t\<^sub>1 = {}" by simp
+  ultimately have "free_vars\<^sub>s (Lam\<^sub>s x t e\<^sub>t\<^sub>1') = {}" by (metis free_vars_eval)
+  hence X: "free_vars\<^sub>s e\<^sub>t\<^sub>1' \<subseteq> insert x (set [])" by simp
+  moreover from ev\<^sub>s_app have Y: "free_vars\<^sub>s v\<^sub>s\<^sub>2 \<subseteq> set []" by simp
+  ultimately have "free_vars\<^sub>s (subst\<^sub>s x v\<^sub>s\<^sub>2 e\<^sub>t\<^sub>1') \<subseteq> set []" by (metis free_vars_subst)
+  with ev\<^sub>s_app X Y show ?case by (simp add: unname_def)
+qed (simp_all add: unname_def)
 
-theorem progresst [simp]: "Map.empty \<turnstile>\<^sub>t e : t \<Longrightarrow> \<exists>v. e \<Down>\<^sub>s v"
+lemma unname_to_app [dest]: "App\<^sub>d e\<^sub>d\<^sub>1 e\<^sub>d\<^sub>2 = unname e\<^sub>t \<Longrightarrow> 
+    \<exists>e\<^sub>t\<^sub>1 e\<^sub>t\<^sub>2. e\<^sub>t = App\<^sub>s e\<^sub>t\<^sub>1 e\<^sub>t\<^sub>2 \<and> e\<^sub>d\<^sub>1 = unname e\<^sub>t\<^sub>1 \<and> e\<^sub>d\<^sub>2 = unname e\<^sub>t\<^sub>2"
+  by (cases e\<^sub>t) (simp_all add: unname_def)
+
+lemma unname_to_lam [dest]: "Lam\<^sub>d t e\<^sub>d = unname e\<^sub>t \<Longrightarrow> 
+    \<exists>x e\<^sub>t'. e\<^sub>t = Lam\<^sub>s x t e\<^sub>t' \<and> e\<^sub>d = unname' [x] e\<^sub>t'"
+  by (cases e\<^sub>t) (simp_all add: unname_def)
+
+theorem complete\<^sub>d [simp]: "unname e\<^sub>t \<Down>\<^sub>d v\<^sub>d \<Longrightarrow> free_vars\<^sub>s e\<^sub>t = {} \<Longrightarrow> \<exists>v\<^sub>t. e\<^sub>t \<Down>\<^sub>s v\<^sub>t \<and> v\<^sub>d = unname v\<^sub>t"
+proof (induction "unname e\<^sub>t" v\<^sub>d arbitrary: e\<^sub>t rule: big_eval\<^sub>d.induct)
+  case (bev\<^sub>d_const n)
+  hence "e\<^sub>t \<Down>\<^sub>s Const\<^sub>s n \<and> Const\<^sub>d n = unname (Const\<^sub>s n)" by (cases e\<^sub>t) (simp_all add: unname_def)
+  thus ?case by fastforce
+next
+  case (bev\<^sub>d_lam t e\<^sub>d)
+  then obtain x e' where "e\<^sub>t = Lam\<^sub>s x t e' \<and> e\<^sub>d = unname' [x] e'" 
+    by (cases e\<^sub>t) (simp_all add: unname_def)
+  hence "e\<^sub>t \<Down>\<^sub>s Lam\<^sub>s x t e' \<and> Lam\<^sub>d t e\<^sub>d = unname (Lam\<^sub>s x t e')" by (simp add: unname_def)
+  thus ?case by fastforce
+next
+  case (bev\<^sub>d_app e\<^sub>d\<^sub>1 t e\<^sub>d\<^sub>1' e\<^sub>d\<^sub>2 v\<^sub>d\<^sub>2 v\<^sub>d)
+  then obtain e\<^sub>t\<^sub>1 e\<^sub>t\<^sub>2 where E: "e\<^sub>t = App\<^sub>s e\<^sub>t\<^sub>1 e\<^sub>t\<^sub>2 \<and> e\<^sub>d\<^sub>1 = unname e\<^sub>t\<^sub>1 \<and> e\<^sub>d\<^sub>2 = unname e\<^sub>t\<^sub>2" 
+    by (cases e\<^sub>t) (simp_all add: unname_def)
+  with bev\<^sub>d_app obtain v\<^sub>t\<^sub>1 where V1: "e\<^sub>t\<^sub>1 \<Down>\<^sub>s v\<^sub>t\<^sub>1 \<and> Lam\<^sub>d t e\<^sub>d\<^sub>1' = unname v\<^sub>t\<^sub>1" by fastforce
+  then obtain x e\<^sub>t\<^sub>1' where X: "v\<^sub>t\<^sub>1 = Lam\<^sub>s x t e\<^sub>t\<^sub>1' \<and> e\<^sub>d\<^sub>1' = unname' [x] e\<^sub>t\<^sub>1'"
+    by (cases v\<^sub>t\<^sub>1) (simp_all add: unname_def)
+  from bev\<^sub>d_app E obtain v\<^sub>t\<^sub>2 where V2: "e\<^sub>t\<^sub>2 \<Down>\<^sub>s v\<^sub>t\<^sub>2 \<and> v\<^sub>d\<^sub>2 = unname v\<^sub>t\<^sub>2" by fastforce
+  from bev\<^sub>d_app E have "free_vars\<^sub>s e\<^sub>t\<^sub>1 = {}" by simp
+  with V1 X have "free_vars\<^sub>s (Lam\<^sub>s x t e\<^sub>t\<^sub>1') = {}" by (metis free_vars_eval)
+  hence Y: "free_vars\<^sub>s e\<^sub>t\<^sub>1' \<subseteq> {x}" by simp
+  from bev\<^sub>d_app E have "free_vars\<^sub>s e\<^sub>t\<^sub>2 = {}" by simp
+  with V2 have Z: "free_vars\<^sub>s v\<^sub>t\<^sub>2 = {}" by auto
+  with Y have "free_vars\<^sub>s (subst\<^sub>s x v\<^sub>t\<^sub>2 e\<^sub>t\<^sub>1') = {}" by (metis free_vars_subst subset_empty)
+  with bev\<^sub>d_app X V2 Y Z have "\<exists>v\<^sub>t. subst\<^sub>s x v\<^sub>t\<^sub>2 e\<^sub>t\<^sub>1' \<Down>\<^sub>s v\<^sub>t \<and> v\<^sub>d = unname v\<^sub>t" 
+    by (simp add: unname_def)
+  then obtain v\<^sub>t where "subst\<^sub>s x v\<^sub>t\<^sub>2 e\<^sub>t\<^sub>1' \<Down>\<^sub>s v\<^sub>t \<and> v\<^sub>d = unname v\<^sub>t" by fastforce
+  with V1 X V2 have "App\<^sub>s e\<^sub>t\<^sub>1 e\<^sub>t\<^sub>2 \<Down>\<^sub>s v\<^sub>t \<and> v\<^sub>d = unname v\<^sub>t" by fastforce
+  with E show ?case by fastforce
+qed
+
+text \<open>Now, finally, we can go back and finish the progress theorems for our typed and source 
+languages. This is the only time we will need to backfill like this; subsequent stages will prove 
+all their relevant metatheoretic properties at once.\<close>
+
+theorem progress\<^sub>t [simp]: "Map.empty \<turnstile>\<^sub>t e\<^sub>t : t \<Longrightarrow> \<exists>v\<^sub>t. e\<^sub>t \<Down>\<^sub>s v\<^sub>t"
 proof -
-  assume X: "Map.empty \<turnstile>\<^sub>t e : t"
-  hence "[] \<turnstile>\<^sub>d convert e : t" by simp
-  then obtain v\<^sub>d where "value\<^sub>d v\<^sub>d \<and> convert e \<Down>\<^sub>d v\<^sub>d" by fastforce
-  with X obtain v\<^sub>n where "e \<Down>\<^sub>s v\<^sub>n \<and> v\<^sub>d = convert v\<^sub>n" by fastforce
+  assume X: "Map.empty \<turnstile>\<^sub>t e\<^sub>t : t"
+  hence "[] \<turnstile>\<^sub>d unname e\<^sub>t : t" by simp
+  then obtain v\<^sub>d where "value\<^sub>d v\<^sub>d \<and> unname e\<^sub>t \<Down>\<^sub>d v\<^sub>d" by fastforce
+  with X obtain v\<^sub>t where "e\<^sub>t \<Down>\<^sub>s v\<^sub>t \<and> v\<^sub>d = unname v\<^sub>t" by fastforce
   thus ?thesis by fastforce
 qed
 
-theorem progressn [simp]: "Map.empty \<turnstile>\<^sub>t e : t \<Longrightarrow> \<exists>v. erase e \<Down>\<^sub>s v"
+theorem progress\<^sub>s [simp]: "\<exists>e\<^sub>t t. erase e\<^sub>t = e\<^sub>s \<and> Map.empty \<turnstile>\<^sub>t e\<^sub>t : t \<Longrightarrow> \<exists>v\<^sub>s. e\<^sub>s \<Down>\<^sub>s v\<^sub>s"
 proof -
-  assume X: "Map.empty \<turnstile>\<^sub>t e : t"
-  then obtain v\<^sub>t where "e \<Down>\<^sub>s v\<^sub>t" by fastforce
-  hence "erase e \<Down>\<^sub>s erase v\<^sub>t" by simp
+  assume "\<exists>e\<^sub>t t. erase e\<^sub>t = e\<^sub>s \<and> Map.empty \<turnstile>\<^sub>t e\<^sub>t : t"
+  then obtain e\<^sub>t t where E: "erase e\<^sub>t = e\<^sub>s \<and> Map.empty \<turnstile>\<^sub>t e\<^sub>t : t" by blast
+  then obtain v\<^sub>t where "e\<^sub>t \<Down>\<^sub>s v\<^sub>t" by fastforce
+  with E have "e\<^sub>s \<Down>\<^sub>s erase v\<^sub>t" by auto
   thus ?thesis by fastforce
 qed
 
